src/hacl.rs
@@ -20,8 +20,7 @@ pub(crate) mod hkdf;
 pub(crate) mod hmac;
 pub(crate) mod p256;
 pub(crate) mod sha2;
-// XXX: Don't make this public when eurydice has improved.
-pub mod sha3;
+pub(crate) mod sha3;
 
 /// Unified error type.
 #[derive(Debug, PartialEq, Eq, Clone, Copy)]
